Move over first batch of stuff (lemmas still missing!)

Hashmap/BEq.lean
@@ -1,39 +1,52 @@
 /-
-Copyright (c) 2024 Lean FRO, LLC. All rights reserved.
+Copyright (c) 2022 Mario Carneiro. All rights reserved.
 Released under Apache 2.0 license as described in the file LICENSE.
-Authors: Markus Himmel
+Authors: Mario Carneiro
 -/
+import Std.Classes.BEq
 
-/-- Class asserting that `BEq` is an equivalence relation. -/
-class EquivBEq (α) [BEq α] : Prop where
-  /-- Reflexitiivty for `BEq`. -/
-  refl : ∀ {a : α}, a == a
-  /-- Symmetry for `BEq`. If `a == b` then `b == a`. -/
-  symm : ∀ {a b : α}, a == b → b == a
-  /-- Transitivity for `BEq`. If `a == b` and `b == c` then `a == c`. -/
-  trans : ∀ {a b c : α}, a == b → b == c → a == c
+/-! ## Boolean equality -/
+
+-- /-- `PartialEquivBEq α` says that the `BEq` implementation is a
+-- partial equivalence relation, that is:
+-- * it is symmetric: `a == b → b == a`
+-- * it is transitive: `a == b → b == c → a == c`.
+-- -/
+-- class PartialEquivBEq (α) [BEq α] : Prop where
+--   /-- Symmetry for `BEq`. If `a == b` then `b == a`. -/
+--   symm : (a : α) == b → b == a
+--   /-- Transitivity for `BEq`. If `a == b` and `b == c` then `a == c`. -/
+--   trans : (a : α) == b → b == c → a == c
+
+/-- `ReflBEq α` says that the `BEq` implementation is reflexive. -/
+class ReflBEq (α) [BEq α] : Prop where
+  /-- Reflexivity for `BEq`. -/
+  refl : (a : α) == a
+
+/-- `EquivBEq` says that the `BEq` implementation is an equivalence relation. -/
+class EquivBEq (α) [BEq α] extends PartialEquivBEq α, ReflBEq α : Prop
 
 @[simp]
-theorem BEq.refl [BEq α] [EquivBEq α] {a : α} : a == a :=
-  EquivBEq.refl
+theorem BEq.refl [BEq α] [ReflBEq α] {a : α} : a == a :=
+  ReflBEq.refl
 
-theorem BEq.symm [BEq α] [EquivBEq α] {a b : α} : a == b → b == a :=
-  EquivBEq.symm
+theorem BEq.symm [BEq α] [PartialEquivBEq α] {a b : α} : a == b → b == a :=
+  PartialEquivBEq.symm
 
-theorem BEq.comm [BEq α] [EquivBEq α] {a b : α} : (a == b) = (b == a) :=
+theorem BEq.comm [BEq α] [PartialEquivBEq α] {a b : α} : (a == b) = (b == a) :=
   Bool.eq_iff_iff.2 ⟨BEq.symm, BEq.symm⟩
 
-theorem BEq.symm_false [BEq α] [EquivBEq α] {a b : α} : (a == b) = false → (b == a) = false :=
+theorem BEq.symm_false [BEq α] [PartialEquivBEq α] {a b : α} : (a == b) = false → (b == a) = false :=
   BEq.comm (α := α) ▸ id
 
-theorem BEq.trans [BEq α] [EquivBEq α] {a b c : α} : a == b → b == c → a == c :=
-  EquivBEq.trans
+theorem BEq.trans [BEq α] [PartialEquivBEq α] {a b c : α} : a == b → b == c → a == c :=
+  PartialEquivBEq.trans
 
-theorem BEq.neq_of_neq_of_beq [BEq α] [EquivBEq α] {a b c : α} :
+theorem BEq.neq_of_neq_of_beq [BEq α] [PartialEquivBEq α] {a b c : α} :
     (a == b) = false → b == c → (a == c) = false := by
   refine fun h₁ h₂ => Bool.eq_false_iff.2 fun h₃ => Bool.eq_false_iff.1 h₁ (BEq.trans h₃ (BEq.symm h₂))
 
-theorem BEq.neq_of_beq_of_neq [BEq α] [EquivBEq α] {a b c : α} :
+theorem BEq.neq_of_beq_of_neq [BEq α] [PartialEquivBEq α] {a b c : α} :
     a == b → (b == c) = false → (a == c) = false := by
   refine fun h₁ h₂ => Bool.eq_false_iff.2 fun h₃ => Bool.eq_false_iff.1 h₂ (BEq.trans (BEq.symm h₁) h₃)
 
