Hashmap/DHashMap/Basic.lean
@@ -1,0 +1,143 @@
+/-
+Copyright (c) 2018 Microsoft Corporation. All rights reserved.
+Released under Apache 2.0 license as described in the file LICENSE.
+Authors: Leonardo de Moura, Mario Carneiro, Markus Himmel
+-/
+import Hashmap.AssocList.Basic
+import Hashmap.LawfulHashable
+import Std.Data.Array.Lemmas
+
+set_option autoImplicit false
+
+universe u v
+
+variable {α : Type u} {β : α → Type v}
+
+namespace MyLean
+
+namespace DHashMap
+
+structure Raw (α : Type u) (β : α → Type v) where
+  size : Nat
+  buckets : Array (AssocList α β)
+
+namespace Raw
+
+private def numBucketsForCapacity (capacity : Nat) : Nat :=
+  -- a "load factor" of 0.75 is the usual standard for hash maps
+  capacity * 4 / 3
+
+def empty (capacity := 8) : Raw α β where
+  size := 0
+  buckets := mkArray (numBucketsForCapacity capacity).nextPowerOfTwo AssocList.nil
+
+private def mkIdx {sz : Nat} (hash : UInt64) (h : 0 < sz) : { u : USize // u.toNat < sz } :=
+  -- TODO: restore this to hash.toUSize &&& (sz.toUSize - 1). This is not so easy because we probably (?) don't want
+  -- to check for m.buckets.size.isPowerOfTwo in Raw.insert, right?
+  ⟨hash.toUSize % sz, Nat.mod_lt _ h⟩
+
+@[inline] def reinsertAux [Hashable α]
+    (data : { d : Array (AssocList α β) // 0 < d.size }) (a : α) (b : β a) : { d : Array (AssocList α β) // 0 < d.size } :=
+  let ⟨data, hd⟩ := data
+  let ⟨i, h⟩ := mkIdx (hash a) hd
+  ⟨data.uset i (data[i].cons a b) h, by simpa⟩
+
+/-- Copies all the entries from `buckets` into a new hash map with a larger capacity. -/
+def expand [Hashable α] (size : Nat) (data : { d : Array (AssocList α β) // 0 < d.size }) : { m : Raw α β // 0 < m.buckets.size } :=
+  let ⟨data, hd⟩ := data
+  let nbuckets := data.size * 2
+  let ⟨newBuckets, hn⟩ := go 0 data ⟨mkArray nbuckets AssocList.nil, by rw [Array.size_mkArray]; exact Nat.mul_pos hd Nat.two_pos⟩
+  ⟨{ size, buckets := newBuckets }, hn⟩
+where
+  /-- Inner loop of `expand`. Copies elements `source[i:]` into `target`,
+  destroying `source` in the process. -/
+  go (i : Nat) (source : Array (AssocList α β)) (target : { d : Array (AssocList α β) // 0 < d.size }) :
+      { d : Array (AssocList α β) // 0 < d.size } :=
+    if h : i < source.size then
+      let idx : Fin source.size := ⟨i, h⟩
+      let es := source.get idx
+      -- We remove `es` from `source` to make sure we can reuse its memory cells
+      -- when performing es.foldl
+      let source := source.set idx .nil
+      let target := es.foldl reinsertAux target
+      go (i+1) source target
+    else target
+  termination_by source.size - i
+
+@[inline] def insertWellFormed [BEq α] [Hashable α] (m : { m : Raw α β // 0 < m.buckets.size }) (a : α) (b : β a) :
+    { m : Raw α β // 0 < m.buckets.size } × Bool :=
+  let ⟨⟨size, buckets⟩, hm⟩ := m
+  let ⟨i, h⟩ := mkIdx (hash a) hm
+  let bkt := buckets[i]
+  if bkt.contains a then
+    (⟨⟨size, buckets.uset i (bkt.replace a b) h⟩, by simpa⟩, true)
+  else
+    let size'    := size + 1
+    let buckets' := buckets.uset i (AssocList.cons a b bkt) h
+    if numBucketsForCapacity size' ≤ buckets.size then
+      (⟨{ size := size', buckets := buckets'}, by simpa [buckets']⟩, false)
+    else
+      (expand size' ⟨buckets', by simpa [buckets']⟩, false)
+
+@[inline] def insert' [BEq α] [Hashable α] (m : Raw α β) (a : α) (b : β a) : Raw α β × Bool :=
+  if h : 0 < m.buckets.size then
+    let ⟨⟨r, _⟩, replaced⟩ := insertWellFormed ⟨m, h⟩ a b
+    ⟨r, replaced⟩
+  else (m, false) -- will never happen for well-formed inputs
+
+@[inline] def insert [BEq α] [Hashable α] (m : Raw α β) (a : α) (b : β a) : Raw α β :=
+  (insert' m a b).1
+
+@[inline] def findEntry?WellFormed [BEq α] [Hashable α] (m : { m : Raw α β // 0 < m.buckets.size }) (a : α) :
+    Option (Σ a, β a) :=
+  let ⟨⟨_, buckets⟩, h⟩ := m
+  let ⟨i, h⟩ := mkIdx (hash a) h
+  buckets[i].findEntry? a
+
+@[inline] def findEntry? [BEq α] [Hashable α] (m : Raw α β) (a : α) : Option (Σ a, β a) :=
+  if h : 0 < m.buckets.size then
+    findEntry?WellFormed ⟨m, h⟩ a
+  else none -- will never happen for well-formed inputs
+
+section WF
+
+def toList (m : Raw α β) : List (Σ a, β a) :=
+  m.buckets.data.bind AssocList.toList
+
+structure IsHashSelf [BEq α] [Hashable α] (m : Raw α β) : Prop where
+  hashes_to (i : Nat) (h : i < m.buckets.size) : m.buckets[i].toList.HashesTo i m.buckets.size
+
+structure WF [BEq α] [Hashable α] (m : Raw α β) extends IsHashSelf m : Prop where
+  buckets_size : m.buckets.size.isPowerOfTwo
+  size_eq : m.size = m.toList.length
+  distinct : m.toList.WF
+
+end WF
+
+end Raw
+
+inductive WF [BEq α] [Hashable α] : Raw α β → Prop where
+  | wf : ∀ m, m.WF → WF m
+  | insert : ∀ m h a b, WF (Raw.insertWellFormed ⟨m, h⟩ a b).1.1
+
+theorem WF.size_buckets_pos [BEq α] [Hashable α] (m : Raw α β) : WF m → 0 < m.buckets.size
+  | wf m h => Nat.pos_of_isPowerOfTwo h.buckets_size
+  | insert m h a b => (Raw.insertWellFormed ⟨m, h⟩ a b).1.2
+
+end DHashMap
+
+def DHashMap (α : Type u) (β : α → Type v) [BEq α] [Hashable α] := { m : DHashMap.Raw α β // DHashMap.WF m }
+
+namespace DHashMap
+
+@[inline] def insert' [BEq α] [Hashable α] (m : DHashMap α β) (a : α) (b : β a) : DHashMap α β × Bool :=
+  let m' := Raw.insertWellFormed ⟨m.1, m.2.size_buckets_pos⟩ a b
+  ⟨⟨m'.1.1, .insert _ _ _ _⟩, m'.2⟩
+
+@[inline] def insert [BEq α] [Hashable α] (m : DHashMap α β) (a : α) (b : β a) : DHashMap α β :=
+  (m.insert' a b).1
+
+@[inline] def findEntry? [BEq α] [Hashable α] (m : DHashMap α β) (a : α) : Option (Σ a, β a) :=
+  Raw.findEntry?WellFormed ⟨m.1, m.2.size_buckets_pos⟩ a
+
+end MyLean.DHashMap
