Hashmap/DHashMap/Lemmas.lean
@@ -1,0 +1,26 @@
+/-
+Copyright (c) 2024 Lean FRO, LLC. All rights reserved.
+Released under Apache 2.0 license as described in the file LICENSE.
+Authors: Markus Himmel
+-/
+import Hashmap.DHashMap.Basic
+
+set_option autoImplicit false
+
+universe u v
+
+variable {α : Type v} {β : α → Type v}
+
+open List
+
+-- TODO
+theorem List.perm_append_comm_assoc (l₁ l₂ l₃ : List α) : l₁ ++ (l₂ ++ l₃) ~ l₂ ++ (l₁ ++ l₃) := by
+  simpa only [List.append_assoc] using perm_append_comm.append_right _
+
+namespace MyLean.DHashMap
+
+namespace Raw
+
+end Raw
+
+end MyLean.DHashMap
